logic.v
@@ -1,0 +1,4 @@
+Theorem contrapositive :
+  forall A B : Prop,
+    (A -> B) <-> ((~B) -> (~A)).
+Proof. Admitted.
